​	

王贤义																计算机基地班                                                                   320210931221

---

将G[S]:S→SS+ | SS* | id 文法转换为

$S'→S$

$S→S_0S_1+$

$S→S_0S_1*$

$S→id$

---

设计的SDD如下所示

产生式  					语法规则

$S'→S$				       $S'.code = S.code$

​								     $print(S'.code)$	

$S→S_0S_1+$			  $S.op="+"$

​								    $if(S_1.op=="+")\ \ then$

​												$S.code = S_0.code+"+"+"("+S_1.code+")"$

​								    $else \ \  \ \ S.code=s_0.code+"+"+S_1.code$

$S→S_0S_1*$			   $S.op="*"$

​									$if((S_0.op=="*" || S_0.op==none) \&\& (S_1.op=="*"||S_1.op=="+")\ then$

​												$S.code=S_0.code+"*"+"("+S_1.code+")"$

​									$else\ \ if(S_0.op=="+"\&\&(S_1.op=="*"||S_1.op=="+"))\ then$

​												$S.code="("+S_0.code+")"+"*"+"("+S_1.code+")"$

​									$else\ \ if((S_0.op=="*"||S_0.op==none)\&\&(S_1.op==none))\ then$

​												$S.code=S_0.code+"*"+S_1.code$

​									$else\ \ if(S_0.op=="+"\&\&S_1.op==none)\ then$

​												$S.code="("+S_0.code+")"+"*"+S_1.code$

$S→id$					   $S.code=id.lexval$

​									$S.op=none$





​					







​				